llist.v
@@ -79,6 +79,9 @@ Section llist.
   Fact lfin_inv a l : lfin (lcons a l) -> lfin l.
   Proof. inversion 1; assumption. Defined.
 
+  Fact lfin_list_llist l : lfin (list_llist l).
+  Proof. induction l; simpl; constructor; trivial. Qed.
+
   Section llist_list.
 
     Let llist_list_rec : forall l, lfin l -> { m | l = list_llist m }.
@@ -99,7 +102,12 @@ Section llist.
   End llist_list.
   
   Arguments llist_list : clear implicits.
-  
+
+  Fact llist_list_eq l H1 H2 : @llist_list l H1 = @llist_list l H2.
+  Proof.
+    apply list_llist_inj; repeat rewrite <- llist_list_spec; trivial.
+  Qed.
+
   Fact llist_list_fix_0 H : llist_list lnil H = nil.
   Proof.
     generalize (llist_list_spec H); simpl.
@@ -134,6 +142,36 @@ Arguments lnil {X}.
 Arguments llist_list {X}.
 Arguments lfin_length {X}.
 
+Section Append.
+
+  Variable (X : Type).
+  
+  Implicit Type (l m : llist X).
+
+  Section def.
+
+    Let llist_app_rec : forall l m (Hl : lfin l) (Hm : lfin m), { k | k = list_llist (llist_list _ Hl ++ llist_list _ Hm) }.
+    Proof.
+      refine (fix loop l m Hl Hm { struct Hl } := _).
+      revert Hl; refine (match l with 
+        | lnil      => fun _  => exist _ m _
+        | lcons x l => fun Hl => let (r,Hr) := loop l m (lfin_inv Hl) Hm in exist _ (lcons x r) _
+      end).
+      + rewrite llist_list_fix_0; simpl; apply llist_list_spec.
+      + rewrite llist_list_fix_1; simpl; f_equal; trivial.
+    Qed.
+
+    Definition llist_app l m Hl Hm := proj1_sig (@llist_app_rec l m Hl Hm).
+
+    Fact llist_app_spec l m Hl Hm : @llist_app l m Hl Hm = list_llist (llist_list _ Hl ++ llist_list _ Hm).
+    Proof. apply (proj2_sig (@llist_app_rec l m Hl Hm)). Qed.
+
+  End def.
+
+  Arguments llist_app : clear implicits.
+
+End Append.
+
 Section Rotate.
 
   (* Rotate with lazy lists (with a non-informative "finiteness" predicate 
@@ -142,41 +180,77 @@ Section Rotate.
 
   Variable (X : Type).
   
-  Implicit Type (f r : llist X) (a : list X).
+  Implicit Type (l r : llist X) (a : llist X).
   
-  Let prec  f Hf r Hr := lfin_length r Hr = 1 + lfin_length f Hf.
-  Let rspec f Hf r Hr a m := m = llist_list f Hf++rev (llist_list r Hr)++a.
-  
-  Fixpoint rotate f r a (Hf : lfin f) (Hr : lfin r) { struct Hf } : @prec f Hf r Hr -> sig (@rspec f Hf r Hr a). 
-  Proof.
-    revert Hr.
-    refine (match r as r' return forall (Hr : lfin r'), @prec f Hf _ Hr  -> sig (@rspec f Hf r' Hr a) with
-      | lnil       => _
-      | lcons y r' => _ 
-    end); intros Hr' H.
-    { exfalso.
-      red in H.
-      rewrite lfin_length_fix_0 in H; discriminate. }
-    revert Hf H.
-    refine (match f as f' return forall (Hf' : lfin f'), @prec f' Hf' _ Hr' -> sig (rspec Hf' Hr' a) with
-      | lnil       => _
-      | lcons x f' => _
-    end); intros Hf' H.
-    + exists (y::a).
-      red in H |- *; revert H.
-      rewrite llist_list_fix_0, llist_list_fix_1, lfin_length_fix_0, lfin_length_fix_1.
-      destruct r'.
-      * rewrite llist_list_fix_0; trivial.
-      * rewrite lfin_length_fix_1; discriminate.
-    + refine (let (ro,Hro) := rotate f' r' (y::a) (lfin_inv Hf') (lfin_inv Hr') _ in exist _ (x::ro) _).
-      * red in H |- *; revert H.
-        repeat rewrite lfin_length_fix_1; intros; omega.
-      * red in Hro |- *; revert Hro.
-        repeat rewrite llist_list_fix_1; intros; subst.
-        simpl; rewrite app_ass; auto.
-  Defined.
+  Section def.
 
+    Let prec  l Hl r Hr := lfin_length r Hr = 1 + lfin_length l Hl.
+    Let rspec l Hl r Hr a Ha m := m = list_llist (llist_list l Hl++rev (llist_list r Hr)++llist_list a Ha).
+  
+    Let llist_rotate_rec : forall l r a Hl Hr Ha, @prec l Hl r Hr -> sig (@rspec l Hl r Hr a Ha).
+    Proof.
+      refine (fix loop l r a Hl Hr Ha { struct Hl } := _). 
+      revert Hr.
+      refine (match r as r' return forall (Hr : lfin r'), @prec l Hl _ Hr  -> sig (@rspec l Hl r' Hr a Ha) with
+        | lnil       => _
+        | lcons y r' => _ 
+      end); intros Hr' H.
+      { exfalso; red in H; rewrite lfin_length_fix_0 in H; discriminate. }
+      revert Hl H.
+      refine (match l as l' return forall (Hl' : lfin l'), @prec l' Hl' _ Hr' -> sig (rspec Hl' Hr' Ha) with
+        | lnil       => _
+        | lcons x l' => _
+      end); intros Hl' H.
+      + exists (lcons y a).
+        red in H |- *; revert H.
+        rewrite llist_list_fix_0, llist_list_fix_1, lfin_length_fix_0, lfin_length_fix_1.
+        destruct r'.
+        * rewrite llist_list_fix_0; simpl. 
+          rewrite <- llist_list_spec; trivial.
+        * rewrite lfin_length_fix_1; discriminate.
+      + refine (let (ro,Hro) := loop l' r' (lcons y a) (lfin_inv Hl') (lfin_inv Hr') (lfin_lcons _ Ha) _ in exist _ (lcons x ro) _).
+        * red in H |- *; revert H.
+          repeat rewrite lfin_length_fix_1; intros; omega.
+        * red in Hro |- *; revert Hro.
+          repeat rewrite llist_list_fix_1; intros; subst.
+          simpl; rewrite app_ass; simpl; auto.
+    Qed.
+
+    Definition llist_rotate f r a Hf Hr Ha H := proj1_sig (@llist_rotate_rec f r a Hf Hr Ha H).
+
+    Fact llist_rotate_spec f r a Hf Hr Ha H : @rspec f Hf r Hr a Ha (@llist_rotate f r a Hf Hr Ha H).
+    Proof. apply (proj2_sig (@llist_rotate_rec f r a Hf Hr Ha H)). Qed.
+
+  End def.
+
+  Arguments llist_rotate : clear implicits.
+
+  Fact lfin_rotate f r a Hf Hr Ha H : lfin (llist_rotate f r a Hf Hr Ha H).
+  Proof.
+    generalize (llist_rotate_spec Ha H); intros E.
+    rewrite E; apply lfin_list_llist.
+  Qed.
+
+  Fact llist_rotate_eq l r a Hl Hr Ha H : llist_list _ (@lfin_rotate l r a Hl Hr Ha H) = llist_list l Hl++rev (llist_list r Hr)++llist_list a Ha.
+  Proof.
+    apply list_llist_inj.
+    rewrite <- (@llist_rotate_spec l r a Hl Hr Ha H).
+    generalize (llist_rotate l r a Hl Hr Ha H) (lfin_rotate Hl Hr Ha H).
+    symmetry; apply llist_list_spec.
+  Qed.
+
+  Fact llist_rotate_length l r a Hl Hr Ha H : lfin_length _ (@lfin_rotate l r a Hl Hr Ha H) = lfin_length _ Hl + lfin_length _ Hr + lfin_length _ Ha.
+  Proof.
+    unfold lfin_length.
+    rewrite llist_rotate_eq.
+    repeat rewrite app_length.
+    rewrite rev_length; omega.
+  Qed.
+ 
 End Rotate.
 
-Recursive Extraction llist_list list_llist rotate.
+Recursive Extraction llist_list list_llist llist_app llist_rotate.
+
+Check llist_rotate.
+Check llist_rotate_spec.
 
